fairness/examples/comp/subtrace.v
@@ -1,0 +1,450 @@
+From trillium.fairness Require Import inftraces fairness.
+From trillium.fairness.examples.comp Require Import lm_fair my_omega lemmas trace_len trace_helpers trace_lookup.
+
+Local Ltac gd t := generalize dependent t.
+
+(* TODO: move*)
+Section Subtrace.
+  Context {St L: Type}.
+  
+
+  CoFixpoint trace_prefix_inf (tr: trace St L) (max_len: nat_omega): trace St L :=
+    match tr, max_len with
+    | tr, NOnum 0 => ⟨ trfirst tr ⟩ (* shouldn't be reached if max_len > 0*)
+    | tr, NOnum 1 => ⟨ trfirst tr ⟩ (* actual base case *)
+    | ⟨ s ⟩, _ => ⟨ s ⟩
+    | s -[ l ]-> tr', ml => s -[l]-> (trace_prefix_inf tr' (NOmega.pred ml))
+    end. 
+
+  Definition subtrace (tr: trace St L) (start: nat) (fin: nat_omega): option (trace St L) :=
+    match (after start tr) with
+    | None => None
+    | Some tr => let max_len := NOmega.sub fin (NOnum start) in
+                if (decide (max_len = NOnum 0))
+                then None
+                else Some (trace_prefix_inf tr max_len)
+    end.
+
+  Lemma trace_prefix_len1 (tr: trace St L):
+    trace_prefix_inf tr (NOnum 1) = ⟨ trfirst tr ⟩.
+  Proof. 
+    rewrite (trace_unfold_fold (trace_prefix_inf tr (NOnum 1))).
+    destruct tr; done. 
+  Qed. 
+
+  Lemma trace_prefix_inf_len (tr: trace St L) (len max_len: nat_omega)
+    (GT0: max_len ≠ NOnum 0)
+    (LEN: trace_len_is tr len)
+    (LE: NOmega.le max_len len)
+    :
+    trace_len_is (trace_prefix_inf tr max_len) max_len.
+  Proof. 
+    destruct max_len.
+    { lia_NO' len.
+      red. simpl. clear -LEN.
+      intros i. gd tr. induction i.
+      { simpl. done. }
+      intros.
+      rewrite (trace_unfold_fold (trace_prefix_inf tr NOinfinity)).
+      destruct tr.
+      { done. }
+      specialize (IHi tr). specialize_full IHi.
+      { apply trace_len_tail in LEN. eauto. }
+      done. }      
+    gd tr. gd len. induction n.
+    { intros. done. }
+    intros. 
+    destruct n. 
+    { rewrite trace_prefix_len1. apply trace_len_singleton. }
+    rewrite (trace_unfold_fold (trace_prefix_inf tr (NOnum (S (S n))))). 
+    destruct tr. 
+    { pose proof (trace_len_singleton s (L := L)) as LEN'.
+      pose proof (trace_len_uniq _ _ _ LEN LEN').
+      subst. simpl in *. lia. }
+    specialize (IHn ltac:(done) (NOmega.pred len)).
+    specialize (IHn ltac:(lia_NO len)). specialize_full IHn.
+    { eapply trace_len_tail; eauto. }
+    apply (trace_len_cons s ℓ) in IHn. done.
+  Qed. 
+
+  (* Lemma trace_prefix_inf_over tr len max_len *)
+  (*   (LEN: trace_len_is tr len) *)
+  (*   (GE: NOmega.le len max_len): *)
+  (*   trace_prefix_inf tr max_len = trace_prefix_inf tr len. *)
+  (* Proof.  *)
+
+  (* Lemma subtrace_over tr start fin len *)
+  (*   (LEN: trace_len_is tr len) *)
+  (*   (GE: NOmega.le len fin): *)
+  (*   subtrace tr start fin = subtrace tr start len. *)
+  (* Proof.  *)
+
+
+  Lemma subtrace_len (tr: trace St L) (len: nat_omega)
+    (start: nat) (fin: nat_omega)
+    (LEN: trace_len_is tr len)
+    (LE: NOmega.lt_nat_l start fin)
+    (BOUND: NOmega.le fin len)
+    :
+    exists str, subtrace tr start fin = Some str /\
+           trace_len_is str (NOmega.sub fin (NOnum start)).
+  Proof. 
+    rewrite /subtrace.
+    forward eapply (proj2 (LEN start)) as [atr SUF]. 
+    { lia_NO' len; lia_NO' fin. }
+    rewrite SUF.
+    destruct decide. 
+    { lia_NO' fin. inversion e. lia. }
+    eexists. split; eauto.
+    eapply trace_prefix_inf_len; eauto.
+    - eapply trace_len_after; eauto.
+    - lia_NO' fin; lia_NO len.
+  Qed.    
+    
+  Lemma trace_prefix_inf_head (tr: trace St L) d:
+    trfirst (trace_prefix_inf tr d) = trfirst tr.
+  Proof.
+    (* rewrite (trace_unfold_fold (trace_prefix_inf tr d)).  *)
+    rewrite (trace_unfold_fold tr).
+    destruct tr, d; simpl; try done.
+    all: by destruct n; [| destruct n]. 
+  Qed. 
+
+  Definition trace_prefix_inf_step_alt tr d :=
+    if (decide (NOmega.le d (NOnum 1)))
+    then ⟨ trfirst tr ⟩
+    else match tr with 
+         | ⟨ s ⟩ => ⟨ s ⟩
+         | s -[ℓ]-> tr' => s -[ℓ]-> trace_prefix_inf tr' (NOmega.pred d)
+         end.
+
+  Definition trace_prefix_inf_step_equiv tr d:
+    trace_prefix_inf tr d = trace_prefix_inf_step_alt tr d.
+  Proof. 
+    rewrite (trace_unfold_fold (trace_prefix_inf tr d)).
+    rewrite /trace_prefix_inf_step_alt. 
+    destruct tr; simpl.
+    - destruct d.
+      + simpl. rewrite decide_False; tauto.
+      + destruct n; [| destruct n].
+        1, 2: rewrite decide_True; [done| ]. 
+        3: rewrite decide_False; [done| ].
+        all: simpl; lia.
+    - destruct d.
+      + rewrite decide_False; [done| ]. tauto.
+      + destruct n; [| destruct n].
+        1, 2: rewrite decide_True; [done| ]. 
+        3: rewrite decide_False; [done| ].
+        all: simpl; lia.
+  Qed.
+
+  Lemma trace_prefix_inf_lookup_bounded
+    (tr : trace St L)
+    (  lim k : nat)
+    (  H : k < lim)
+    (  len : nat_omega)
+    (  LEN : trace_len_is tr len)
+    (  BOUND : NOmega.lt_nat_l lim len):
+    trace_prefix_inf tr (NOnum lim) S!! k = tr S!! k /\
+      (k < lim - 1 -> trace_prefix_inf tr (NOnum lim) !! k = tr !! k). 
+  Proof.
+    gd lim. gd tr. gd len. induction k.  
+    { intros.
+      rewrite trace_prefix_inf_step_equiv. 
+      rewrite /trace_prefix_inf_step_alt. simpl.  
+      destruct decide.
+      - assert (lim = 1) as -> by lia.
+        destruct tr; try done. simpl.
+        split; [| lia].
+        done.
+      - split; [by destruct tr| ].
+        intros. destruct tr; [done| ].
+        rewrite trace_lookup_0_cons.
+        by rewrite trace_prefix_inf_head. } 
+    intros.
+    rewrite trace_prefix_inf_step_equiv.
+    rewrite /trace_prefix_inf_step_alt.
+    destruct decide.
+    - simpl in l. assert (lim = 1) as -> by lia.
+      lia.
+    - simpl in *. destruct tr.
+      + pose proof (trace_len_singleton s (L := L)) as LEN'. 
+        forward eapply (trace_len_uniq _ _ _ LEN LEN') as ->.
+        simpl in *. lia.
+      + rewrite !trace_lookup_cons !state_lookup_cons.
+        destruct lim; [lia| ].
+        rewrite PeanoNat.Nat.sub_succ_l; [| lia].
+        setoid_rewrite <- Nat.succ_lt_mono. 
+        eapply IHk; eauto.
+        { apply trace_len_tail in LEN. eauto. }
+        { lia. }
+        lia_NO' len. 
+  Qed. 
+
+  Lemma trace_prefix_inf_lookup_unbounded
+(  tr : trace St L)
+(  d : nat_omega)
+(  k : nat)
+(  H : NOmega.lt_nat_l k d)
+(  len : nat_omega)
+(  LEN : trace_len_is tr len)
+(  LE : NOmega.le len d):
+  trace_prefix_inf tr d !! k = tr !! k.
+  Proof. 
+    gd d. gd tr. gd len. induction k.  
+    { intros.
+      rewrite trace_prefix_inf_step_equiv.
+      rewrite /trace_prefix_inf_step_alt. 
+      destruct decide.
+      - lia_NO' d. assert (n = 1) as -> by lia.
+        lia_NO' len. assert (n = 0 \/ n = 1) as [-> | ->] by lia.
+        + by apply trace_len_0_inv in LEN.
+        + apply trace_len_1_inv in LEN as [? ->]. done.
+      - destruct tr; try done.
+        rewrite !trace_lookup_0_cons.
+        by rewrite trace_prefix_inf_head. }
+    intros.
+    rewrite trace_prefix_inf_step_equiv.
+    rewrite /trace_prefix_inf_step_alt.
+    destruct decide.
+    - lia_NO' d.
+    - destruct tr.
+      { lia_NO' d. }
+      rewrite !trace_lookup_cons. eapply IHk; eauto.
+      { apply trace_len_tail in LEN. apply LEN. }
+      { lia_NO d. }
+      lia_NO' len; lia_NO' d.
+  Qed. 
+  
+  Lemma trace_prefix_inf_lookup tr d:
+    forall k, NOmega.lt_nat_l k d ->
+         trace_prefix_inf tr d S!! k = tr S!! k /\
+         (NOmega.lt_nat_l (k + 1) d -> trace_prefix_inf tr d !! k = tr !! k). 
+  Proof.
+    intros.
+    pose proof (trace_has_len tr) as [len LEN].
+    destruct (decide (NOmega.le len d)) as [LE | LT].
+    { forward eapply trace_prefix_inf_lookup_unbounded as KTH; eauto.
+      split; eauto.
+      rewrite /state_lookup.
+      rewrite /lookup /trace_lookup in KTH.
+      by rewrite KTH. }      
+    
+    assert (exists lim, d = NOnum lim /\ NOmega.lt_nat_l lim len)
+             as (lim & -> & BOUND). 
+    { lia_NO' len; lia_NO' d; eauto.
+      exists n0. split; eauto. lia. }
+    simpl in *.
+    setoid_rewrite Nat.lt_add_lt_sub_r. 
+    eapply trace_prefix_inf_lookup_bounded; eauto.
+  Qed. 
+    
+  (* Lemma subtrace_lookup_after (tr: trace St L) str atr *)
+  (*   (start: nat) (fin: nat_omega) *)
+  (*   (SUB: subtrace tr start fin = Some str) *)
+  (*   (AFTER: after start tr = Some atr): *)
+  (*   forall k, str !! k = atr !! k.  *)
+  (* Proof.  *)
+
+  Lemma subtrace_lookup (tr: trace St L) str
+    (start: nat) (fin: nat_omega)
+    (SUB: subtrace tr start fin = Some str):
+    forall k, NOmega.lt_nat_l k (NOmega.sub fin (NOnum start)) ->
+         str S!! k = tr S!! (start + k) /\
+         (NOmega.lt_nat_l (k + 1) (NOmega.sub fin (NOnum start)) -> 
+          str !! k = tr !! (start + k)). 
+  Proof. 
+    intros.
+    rewrite /subtrace in SUB.
+    destruct (after start tr) eqn:AFTER; [| done].
+    destruct decide; [done| ].
+    inversion SUB. subst. clear SUB. 
+    erewrite <- trace_lookup_after; [| apply AFTER].
+    erewrite <- state_lookup_after; [| apply AFTER].
+    eapply trace_prefix_inf_lookup.
+    lia_NO fin. 
+  Qed.
+
+  (* TODO: move *)
+  Require Import Coq.Logic.Classical.
+
+  Lemma trace_prop_split (tr: trace St L) (P: (St * option (L * St)) -> Prop) len 
+    (DECP: forall res, Decision (P res))
+    (LEN: trace_len_is tr len)
+    : 
+    exists (l: nat_omega), 
+    (forall i res (LT: NOmega.lt (NOnum i) l) (RES: tr !! i = Some res), P res) /\
+    (forall j res (NEXT: l = NOnum j) (RES: tr !! j = Some res), ¬ P res) /\
+    NOmega.le l len. 
+  Proof using.
+    destruct (classic (exists j res, tr !! j = Some res /\ ¬ P res)) as [STOP | EV]. 
+    - destruct STOP as [j' STOP'].
+      pattern j' in STOP'. apply min_prop_dec in STOP' as [j [NPROP MIN]]. 
+      2: { intros. admit. }
+      exists (NOnum j). simpl in *. repeat split.      
+      + intros. destruct (decide (P res)); [done| ]. 
+        enough (j <= i); [lia| ].
+        apply MIN. eexists. split; eauto.
+      + intros. inversion NEXT. subst.
+        destruct NPROP as [? [RES' NP]].
+        congruence.
+      + lia_NO' len.
+        destruct NPROP as [? [RES' NP]].
+        pose proof (proj1 (trace_lookup_dom _ _ LEN j) (ex_intro _ x RES')).
+        simpl in H. lia. 
+    - exists len. repeat split.
+      + intros.
+        apply not_exists_forall_not with (x := i) in EV. 
+        apply not_exists_forall_not with (x := res) in EV.
+        apply not_and_or in EV. destruct EV; [done| ].
+        eapply NNP_P; eauto.
+      + intros.
+        apply not_exists_forall_not with (x := j) in EV.        
+        pose proof (proj1 (trace_lookup_dom _ _ LEN j)).
+        specialize (H ltac:(eauto)).
+        lia_NO' len. inversion NEXT. lia.
+      + lia_NO len. 
+  Admitted. 
+
+  Lemma trace_prop_split' (tr: trace St L) (P: (St * option (L * St)) -> Prop) 
+    len
+    (start: nat)
+    (DECP: forall res, Decision (P res))
+    (LEN: trace_len_is tr len)
+    (BOUND: NOmega.le (NOnum start) len)
+    : 
+    exists (l: nat_omega),      
+    (forall i res (GE: start <= i) (LT: NOmega.lt (NOnum i) l) (RES: tr !! i = Some res), P res) /\
+    (forall j res (NEXT: l = NOnum j) (RES: tr !! j = Some res), ¬ P res) /\
+    NOmega.le (NOnum start) l /\
+    NOmega.le l len.
+  Proof using.
+    destruct (after start tr) eqn:AFTER.
+    2: { eapply trace_len_neg in AFTER; eauto.
+         assert (len = NOnum start) as ->.
+         { lia_NO' len. f_equal. lia. }
+         exists (NOnum start). repeat split.
+         3, 4: done. 
+         - intros. eapply mk_is_Some in RES.
+           apply (trace_lookup_dom _ _ LEN) in RES.
+           simpl in *. lia.
+         - intros. inversion NEXT. subst j.
+           eapply mk_is_Some in RES.
+           apply (trace_lookup_dom _ _ LEN) in RES.
+           simpl in *. lia. }
+    forward eapply (trace_prop_split t).
+    { eauto. }
+    { eapply trace_len_after in AFTER; eauto. }
+    intros (l&L1&L2&LE).
+    exists (NOmega.add l (NOnum start)). repeat split.
+    - intros. apply Nat.le_sum in GE as [d ->].
+      apply (L1 d); eauto.
+      + lia_NO l.
+      + erewrite trace_lookup_after; eauto.
+    - intros.
+      lia_NO' l. inversion NEXT. subst j. clear NEXT.
+      eapply L2; eauto.
+      rewrite Nat.add_comm in RES. 
+      erewrite trace_lookup_after; eauto.
+    - lia_NO l. 
+    - lia_NO' l; lia_NO' len.
+  Qed.     
+
+
+  Lemma subtrace_inv tr len str start max_len
+    (SUB: subtrace tr start max_len = Some str)
+    (LEN: trace_len_is tr len):
+    NOmega.lt_nat_l start max_len /\ NOmega.lt_nat_l start len.
+  Proof. 
+    rewrite /subtrace in SUB.
+    destruct (after start tr) eqn:AFTER.
+    2: { done. } 
+    destruct decide; [done| ].
+    inversion SUB. subst. clear SUB.
+    eapply mk_is_Some, LEN in AFTER.
+    split; auto.
+    lia_NO' max_len. 
+    destruct (decide (start < n0)); [done| ].
+    destruct n. f_equal. lia.
+  Qed. 
+
+  (* TODO: is it possible to show their equality? *)
+  (* also possible to generalize to any max_len >= len(tr) *)
+  Lemma inf_subtrace_after_lookup (tr str atr: trace St L) k
+    (SUB: subtrace tr k NOinfinity = Some str)
+    (AFTER: after k tr = Some atr):
+    forall k, str !! k = atr !! k.
+  Proof. 
+    intros.
+    erewrite (trace_lookup_after tr atr); eauto.
+    eapply subtrace_lookup; done. 
+  Qed. 
+
+End Subtrace.
+
+
+Section ModelSubtrace.
+  Context {St L: Type}. 
+
+  Lemma fair_by_subtrace
+    (tr str: trace St (option L)) k P
+    (SUB: subtrace tr k NOinfinity = Some str)
+    (FAIR: ∀ ρ, fair_by P ρ tr):
+    ∀ ρ, fair_by P ρ str.
+  Proof. 
+    intros.
+    pose proof (trace_has_len tr) as [len LEN]. 
+    forward eapply subtrace_inv as [_ BOUND]; eauto.
+    apply LEN in BOUND as [atr AFTER]. 
+    eapply (fair_by_after P ρ tr atr) in FAIR; eauto.
+    red. intros.
+    apply pred_at_trace_lookup' in H as (s & step & NTH & Ps).
+    red in FAIR. specialize (FAIR n). specialize_full FAIR.
+    { apply pred_at_trace_lookup'.
+      erewrite <- inf_subtrace_after_lookup; eauto. }
+    destruct FAIR as [m FAIR]. exists m.
+    apply pred_at_or. apply pred_at_trace_lookup'. 
+    apply pred_at_or in FAIR.
+    apply pred_at_trace_lookup' in FAIR as (s'&step'&MNth&PROP).
+    erewrite inf_subtrace_after_lookup; eauto.
+  Qed.
+  
+  
+  From Paco Require Import paco1 paco2 pacotac.
+  (* TODO: merge with mtrace_valid_steps'*)
+  Lemma trace_valid_equiv `{M: FairModel} (tr: mtrace M)
+    (VALID': forall i s1 ℓ s2, tr !! i = Some (s1, Some (ℓ, s2)) ->
+                          fmtrans _ s1 ℓ s2):
+    mtrace_valid tr. 
+  Proof. 
+    pcofix V.
+    intros; pfold.
+    rewrite (trace_unfold_fold tr); simpl.
+    destruct tr.
+    { constructor. }
+  Admitted.
+  
+  
+  (* TODO: move *)
+  Lemma subtrace_valid `{M: FairModel} (tr: mtrace M) len
+    str start max_len
+    (LEN: trace_len_is tr len)
+    (VALID: mtrace_valid tr)
+    (BOUND: NOmega.le max_len len) (* TODO: relax? *)
+    (SUB2: subtrace tr start max_len = Some str):
+    mtrace_valid str.
+  Proof.
+    forward eapply subtrace_inv as [LT1 LT2]; eauto.
+    apply trace_valid_equiv. intros.
+    eapply mtrace_valid_steps' in VALID; eauto.
+    rewrite -H. symmetry.
+    forward eapply (subtrace_len tr _ _ max_len); eauto.
+    intros (str' & SUB' & LEN').
+    assert (str' = str) as -> by congruence.
+    assert (NOmega.lt_nat_l (i + 1) (NOmega.sub max_len (NOnum start))) as LT'.
+    { eapply trace_lookup_dom_strong; eauto. }
+    eapply subtrace_lookup; eauto.
+    lia_NO max_len. 
+  Qed. 
+
+End ModelSubtrace.
